

1 Disformal Transformation

1.1 Perturbing the FLRW Metric

Let us decompose the perturbed FLRW metric (with SVT decomposition) as

$$ds^2 = -(1+2\varphi) dt^2 + 2a(\alpha_{;i} + \beta_i) dt dx^i + a^2 \left[(1-2\psi)\delta_{ij} + \gamma_{ij} + 2E_{;ij} + 2F_{(i,j)} \right] dx^i dx^j, \quad (1.1)$$

where $a = a(t)$ is the scale factor, $(\varphi, \alpha, \psi, E)$ are scalar perturbations, β_i, F_i are vector perturbations, and γ_{ij} are tensor perturbations.

Under a disformal transformation, the line element becomes

$$d\hat{s}^2 = \hat{g}_{\mu\nu} dx^\mu dx^\nu. \quad (1.2)$$

The invertible disformal transformation with higher derivatives presented by Takahashi, Motohashi, and Minamitsuji (which we call the TMM transformation for convenience) is

$$\hat{g}_{\mu\nu} = A g_{\mu\nu} + B \phi_{;\mu} \phi_{;\nu} + C (\phi_{;\mu} X_{;\nu} + X_{;\mu} \phi_{;\nu}) + D X_{;\mu} X_{;\nu}, \quad (1.3)$$

where A, B, C, D are functionals of ϕ, X, Y, Z , and X, Y, Z are defined as

$$X \equiv -\frac{1}{2} g^{\mu\nu} \phi_{;\mu} \phi_{;\nu}, \quad Y \equiv g^{\mu\nu} \phi_{;\mu} X_{;\nu}, \quad Z \equiv g^{\mu\nu} X_{;\mu} X_{;\nu}. \quad (1.4)$$

The TMM form can be simplified by a “completing-the-square” step. We have “squared” covariant-derivative terms of ϕ , cross terms in the middle, and “squared” covariant-derivative terms of X . Recall the elementary identity

$$ax^2 + 2bxy + cy^2 = a \left(x + \frac{b}{a} y \right)^2 + \left(c - \frac{b^2}{a} \right) y^2. \quad (1.5)$$

Identifying $a = B$, $b = C$, and $c = D$, the last three terms in (1.3) combine as

$$B \left(\phi_{;\mu} + \frac{C}{B} X_{;\mu} \right) \left(\phi_{;\nu} + \frac{C}{B} X_{;\nu} \right) + \left(D - \frac{C^2}{B} \right) X_{;\mu} X_{;\nu}. \quad (1.6)$$

Hence, (1.3) may be rewritten as

$$\hat{g}_{\mu\nu} = A g_{\mu\nu} + B \left(\phi_{;\mu} + \frac{C}{B} X_{;\mu} \right) \left(\phi_{;\nu} + \frac{C}{B} X_{;\nu} \right) + \left(D - \frac{C^2}{B} \right) X_{;\mu} X_{;\nu}. \quad (1.7)$$

If we define

$$\Phi_\mu \equiv \sqrt{B} \left(\phi_{;\mu} + \frac{C}{B} X_{;\mu} \right), \quad \Delta \equiv D - \frac{C^2}{B}, \quad (1.8)$$

then the transformation reduces cleanly to

$$\boxed{\hat{g}_{\mu\nu} = A g_{\mu\nu} + \Phi_\mu \Phi_\nu + \Delta X_{;\mu} X_{;\nu}.} \quad (1.9)$$

Under (1.9), the transformed line element can be expanded as

$$\begin{aligned} d\hat{s}^2 &= \hat{g}_{\mu\nu} dx^\mu dx^\nu \\ &= (A g_{00} + \Phi_0 \Phi_0 + \Delta X_{;0} X_{;0}) dt^2 \\ &\quad + 2(A g_{0i} + \Phi_0 \Phi_i + \Delta X_{;0} X_{;i}) dt dx^i \\ &\quad + (A g_{ij} + \Phi_i \Phi_j + \Delta X_{;i} X_{;j}) dx^i dx^j. \end{aligned} \quad (1.10)$$

Consequently, take the perturbed scalar field $\phi = \bar{\phi} + \delta\phi$. Then

$$\begin{aligned}
X &= -\frac{1}{2}g^{\mu\nu}\phi_{;\mu}\phi_{;\nu} \\
&= -\frac{1}{2}g^{00}\dot{\phi}^2 \\
&= -\frac{1}{2}(-(1-2\varphi))(\dot{\bar{\phi}} + \delta\dot{\phi})^2 \\
&= \left(\frac{1}{2} - \varphi\right)(\dot{\bar{\phi}}^2 + 2\dot{\bar{\phi}}\delta\dot{\phi} + (\delta\dot{\phi})^2) \\
&= \frac{1}{2}\dot{\bar{\phi}}^2 + \dot{\bar{\phi}}\delta\dot{\phi} - \varphi\dot{\bar{\phi}}^2,
\end{aligned} \tag{1.11}$$

where g^{00} comes from the perturbed metric, and we have dropped higher-order perturbations (e.g. $(\delta\dot{\phi})^2$).

It is natural to split A , Φ_0 , and Δ as

$$A = \bar{A} + \delta A, \quad \Phi_0 = \bar{\Phi}_0 + \delta\Phi_0, \quad \Delta = \bar{\Delta} + \delta\Delta, \tag{1.12}$$

Notice that from (1.8) we have

$$\begin{aligned}
\Phi_0 &= \sqrt{B}\left(\phi_{;0} + \frac{C}{B}X_{;0}\right) \\
&= \sqrt{B}\left(\dot{\bar{\phi}} + \delta\dot{\phi} + \frac{C}{B}(\dot{\bar{X}} + \delta\dot{X})\right)
\end{aligned} \tag{1.13}$$

Where we see to have zeroth order perturbations given back the background variables. On the other hand for the spatial component, notice

$$\begin{aligned}
\Phi_i &= \sqrt{B}\left(\phi_{;i} + \frac{C}{B}X_{;i}\right) \\
&= \sqrt{B}\left(\frac{C}{B}(\bar{X}_{;i} + \delta X_{;i})\right) \\
&= \sqrt{B}\left(\frac{C}{B}\delta X_{;i}\right)
\end{aligned} \tag{1.14}$$

Where again, the background term vanishes under a spatial covariant derivative since it is only dependent upon time. On the other hand, we are left with $\delta X_{;i}$ which is a first order perturbation. Hence, we choose not to "split" the spatial components of Φ_μ

1.2 For the dt^2 terms

From the perturbed metric given by (1.1) we have $g_{00} = -(1-2\varphi)$ it follows that

$$\begin{aligned}
Ag_{00} &= -(\bar{A} + \delta A)(1-2\varphi) \\
&= -(\bar{A} + 2\varphi\bar{A} + \delta A + 2\varphi\delta A) \\
&\approx -\bar{A} - \delta A - 2\bar{A}\varphi
\end{aligned} \tag{1.15}$$

On the other hand

$$\Phi_0^2 = (\bar{\Phi}_0 + \delta\Phi_0)^2 = \bar{\Phi}_0^2 + 2\bar{\Phi}_0\delta\Phi_0 \tag{1.16}$$

Finally,

$$\begin{aligned}
\Delta X_{;0} X_{;0} &= (\bar{\Delta} + \delta\Delta)(\dot{\bar{X}} + \delta X)^2 \\
&= (\bar{\Delta} + \delta\Delta)(\dot{\bar{X}}^2 + 2\dot{\bar{X}}\delta X + \underbrace{(\delta X)^2}_{\text{2nd order}}) \\
&\approx \bar{\Delta}\dot{\bar{X}}^2 + \delta\Delta\dot{\bar{X}}^2 + 2\bar{\Delta}\dot{\bar{X}}\delta X + \underbrace{2\delta\Delta\dot{\bar{X}}\delta X}_{\text{2nd order}} \\
&\approx \bar{\Delta}\dot{\bar{X}}^2 + \delta\Delta\dot{\bar{X}}^2 + 2\bar{\Delta}\dot{\bar{X}}\delta X
\end{aligned} \tag{1.17}$$

1.3 For $dt dx^i$ terms

Again, given by (1.1) we find that $g_{0i} = a(\alpha_{,i} + \beta_i)$. So for Ag_{0i} we have

$$\begin{aligned}
Ag_{0i} &= a(\bar{A} + \delta A)(\alpha_{,i} + \beta_i) \\
&= a(\bar{A}\alpha_{,i} + \bar{A}\beta_i + \delta A\alpha_{,i} + \delta A\beta_i) \\
&\approx a\bar{A}(\alpha_{,i} + \beta_i)
\end{aligned} \tag{1.18}$$

For $\Phi_0\Phi_i$ note that we have already established that Φ_i is already a first order perturbation. Then

$$\begin{aligned}
\Phi_0\Phi_i &= (\bar{\Phi}_0 + \delta\Phi_0)(\Phi_i) \\
&= \bar{\Phi}_0\Phi_i + \delta\Phi_0\Phi_i \\
&\approx \bar{\Phi}_0\Phi_i
\end{aligned} \tag{1.19}$$

On the other hand, for $\Delta X_{;0} X_{;i}$, note that $X_{;i} = \bar{X}_{;i} + \delta X_{;i} = \delta X_{;i}$ since background quantities are only time dependent. So,

$$\begin{aligned}
\Delta X_{;0} X_{;i} &= (\bar{\Delta} + \delta\Delta)(\bar{X}_{;0} + \delta X_{;0})\delta X_{;i} \\
&= (\bar{\Delta}\dot{\bar{X}} + \bar{\Delta}\delta\dot{\bar{X}} + \delta\Delta\dot{\bar{X}} + \delta\Delta\delta\dot{\bar{X}})\delta X_{;i} \\
&\approx (\bar{\Delta}\dot{\bar{X}} + \bar{\Delta}\delta\dot{\bar{X}} + \delta\Delta\dot{\bar{X}})\delta X_{;i} \\
&\approx \bar{\Delta}\dot{\bar{X}}\delta X_{;i}
\end{aligned} \tag{1.20}$$

1.4 For $dx^i dx^j$ terms